completeness consequences

theories/Core/Completeness/Consequences/Types.v
@@ -55,7 +55,7 @@ Hint Resolve typ_eq_sort_implies_eq_level : mcpts.
 Inductive is_typ_constr {P} : typ P -> Prop :=
 | typ_is_typ_constr : forall s, is_typ_constr {{{ Sort@s }}}
 | nat_is_typ_constr : is_typ_constr {{{ ℕ }}}
-| pi_is_typ_constr : forall s1 s2 s3 (r : Ru P s1 s2 s3) A B, is_typ_constr {{{ Π r A B }}}
+| pi_is_typ_constr : forall s1 s2 s3 (r : Ru_pi P s1 s2 s3) A B, is_typ_constr {{{ Π r A B }}}
 | var_is_typ_constr : forall x, is_typ_constr {{{ #x }}}
 .
 
@@ -84,12 +84,12 @@ Proof.
   unfold per_sort in *.
   destruct_conjs.
   
-  assert (exists A' s', {{ #x : A'@s'  ∈ Γ }} /\ {{ Γ ⊢ A' ≈ Sort@s }}) as [A' [s' [? _]]] by mauto 2.
+  assert (exists A' s', {{ #x : A'@s'  ∈ Γ }} /\ {{ Γ ⊢ A' ⊆ Sort@s }}) as [A' [s' [? _]]] by mauto 2.
   assert (exists a, {{ #| ρ[x] |↘ ⇑! a (length Γ - x - 1) }}) as [? Heq] by mauto 2.
   destruct Histyp;
     invert_rel_typ_body.
   (* unfold per_bot in H5. *)
-  assert (exists A'' s'', {{ #x1 : A''@s''  ∈ Γ }} /\ {{ Γ ⊢ A'' ≈ Sort@s }}) as [A'' [s'' [? _]]] by mauto 2.
+  assert (exists A'' s'', {{ #x1 : A''@s''  ∈ Γ }} /\ {{ Γ ⊢ A'' ⊆ Sort@s }}) as [A'' [s'' [? _]]] by mauto 2.
   assert (exists a', {{ #| ρ[x1] |↘ ⇑! a' (length Γ - x1 - 1) }}) as [? Heq'] by mauto 2.
   assert (x < length Γ) by mauto 2.
   assert (x1 < length Γ) by mauto 2.  
@@ -123,8 +123,8 @@ Proof.
   gen_presups.
   
   inversion_clear HB.
-  assert (exists A' s', {{ #x : A'@s'  ∈ Γ }} /\ {{ Γ ⊢ A' ≈ Sort@s }}) as [A' [s' [? ?]]] by mauto 2.
-  assert (exists a, {{ #| ρ[x] |↘ ⇑! a (length Γ - x - 1) }}) as [? Heq] by mauto 2.
+  assert (exists A' s', {{ #x : A'@s'  ∈ Γ }} /\ {{ Γ ⊢ A' ⊆ Sort@s }}) as [A' [s' [? ?]]] by mauto 2.
+  assert (exists a, {{ #| ρ[x] |↘ ⇑! a (length Γ - x - 1) }}) as [? Heq] by mauto 2.  
   simplify_evals.
 
   dependent destruction H6.
@@ -136,20 +136,109 @@ Proof.
     invert_rel_typ_body.
   
   inversion_clear HA.
-  assert (exists A'' s'', {{ #x2 : A''@s''  ∈ Γ }} /\ {{ Γ ⊢ A'' ≈ Sort@s1 }}) as [A'' [s'' [? ?]]] by mauto 2.
-  assert (exists a', {{ #| ρ[x2] |↘ ⇑! a' (length Γ - x2 - 1) }}) as [? Heq'] by mauto 2.
+  assert (exists A'' s'', {{ #x3 : A''@s''  ∈ Γ }} /\ {{ Γ ⊢ A'' ⊆ Sort@s1 }}) as [A'' [s'' [? ?]]] by mauto 2.
+  assert (exists a', {{ #| ρ[x3] |↘ ⇑! a' (length Γ - x3 - 1) }}) as [? Heq'] by mauto 2.
   simplify_evals.
-  assert (x2 < length Γ) by mauto 2.
-  assert (x1 < length Γ) by mauto 2.  
+  assert (x3 < length Γ) by mauto 2.
+  assert (x2 < length Γ) by mauto 2.  
   f_equal.
-  enough (length Γ - x2 - 1 = length Γ - x1 - 1) by lia.
+  enough (length Γ - x3 - 1 = length Γ - x2 - 1) by lia.
   inversion H13.
   lia.
 Qed.
 
 #[export]
-Hint Resolve is_typ_constr_and_typ_eq_var_implies_eq_var : mcpts.
+  Hint Resolve is_typ_constr_and_typ_eq_var_implies_eq_var : mcpts.
 
+Theorem is_typ_constr_and_var_subtyp_typ_implies_eq_var {P} (pred_P : PredicativeSig P) : forall (Γ : ctx P) x A,
+    is_typ_constr A ->
+    {{ Γ ⊢ #x ⊆ A }} ->
+    exists x', A = {{{ #x' }}}.
+Proof.
+  intros * Histyp ?.
+  assert {{ ⟪ pred_P ⟫ Γ ⊨ #x ⊆ A }} as [env_relΓ] by mauto using completeness_fundamental_typ_subtyp.
+  destruct_conjs.
+  assert (exists p p', initial_env Γ p /\ initial_env Γ p' /\ {{ Dom p ≈ p' ∈ env_relΓ }}) as [ρ [ρ' []]]by mauto using per_ctx_then_per_env_initial_env.
+  destruct_conjs.
+  functional_initial_env_rewrite_clear.
+  (on_all_hyp: destruct_rel_by_assumption env_relΓ).
+  destruct_by_head (@rel_typ_unsorted P).
+  invert_rel_typ_body.
+  destruct_by_head (@rel_exp).
+  gen_presups.
+  
+  inversion_clear HA.
+  assert (exists A' s', {{ #x : A'@s'  ∈ Γ }} /\ {{ Γ ⊢ A' ⊆ Sort@s }}) as [A' [s' [? ?]]] by mauto 2.
+  assert (exists a, {{ #| ρ[x] |↘ ⇑! a (length Γ - x - 1) }}) as [? Heq] by mauto 2.  
+  destruct Histyp; simplify_evals; inversion_clear H10.
+
+  - destruct (per_subtyp_sort_inv_right pred_P H9) as [s'' []].
+    inversion H6.
+  - inversion_clear H8.
+    invert_per_sort_elem H5.
+    pose proof (per_subtyp_nat_inv_right pred_P H9).
+    inversion H8.
+  - invert_per_sort_elem H6.
+    destruct (per_subtyp_pi_inv_right pred_P H9) as [a' [ρ' [B']]].
+    inversion H10.
+  - inversion_clear HB.
+    assert (exists A'' s'', {{ #x1 : A''@s''  ∈ Γ }} /\ {{ Γ ⊢ A'' ⊆ Sort@s1 }}) as [A'' [s'' [? ?]]] by mauto 2.
+    assert (exists a, {{ #| ρ[x1] |↘ ⇑! a (length Γ - x1 - 1) }}) as [? Heq] by mauto 2.
+    simplify_evals.
+
+    assert (x < length Γ) by mauto 2. 
+    assert (x1 < length Γ) by mauto 2.
+    eexists.
+    f_equal.
+Qed.
+
+#[export]
+  Hint Resolve is_typ_constr_and_var_subtyp_typ_implies_eq_var : mcpts.
+
+Theorem is_typ_constr_and_typ_subtyp_var_implies_eq_var {P} (pred_P : PredicativeSig P) : forall (Γ : ctx P) x A,
+    is_typ_constr A ->
+    {{ Γ ⊢ A ⊆ #x }} ->
+    exists x', A = {{{ #x' }}}.
+Proof.
+  intros * Histyp ?.
+  assert {{ ⟪ pred_P ⟫ Γ ⊨ A ⊆ #x }} as [env_relΓ] by mauto using completeness_fundamental_typ_subtyp.
+  destruct_conjs.
+  assert (exists p p', initial_env Γ p /\ initial_env Γ p' /\ {{ Dom p ≈ p' ∈ env_relΓ }}) as [ρ [ρ' []]]by mauto using per_ctx_then_per_env_initial_env.
+  destruct_conjs.
+  functional_initial_env_rewrite_clear.
+  (on_all_hyp: destruct_rel_by_assumption env_relΓ).
+  destruct_by_head (@rel_typ_unsorted P).
+  invert_rel_typ_body.
+  destruct_by_head (@rel_exp).
+  gen_presups.
+  
+  inversion_clear HB.
+  assert (exists A' s', {{ #x : A'@s'  ∈ Γ }} /\ {{ Γ ⊢ A' ⊆ Sort@s }}) as [A' [s' [? ?]]] by mauto 2.
+  assert (exists a, {{ #| ρ[x] |↘ ⇑! a (length Γ - x - 1) }}) as [? Heq] by mauto 2.  
+  destruct Histyp; simplify_evals; inversion_clear H8.
+
+  - destruct (per_subtyp_sort_inv_left pred_P H9) as [s'' []].
+    inversion H6.
+  - inversion_clear H10.
+    invert_per_sort_elem H3.
+    epose proof (per_subtyp_nat_inv_left pred_P H9).
+    inversion H8.
+  - invert_per_sort_elem H6.
+    destruct (per_subtyp_pi_inv_left pred_P H9) as [a' [ρ' [B']]].
+    inversion H8 .
+  - inversion_clear HA.
+    assert (exists A'' s'', {{ #x1 : A''@s''  ∈ Γ }} /\ {{ Γ ⊢ A'' ⊆ Sort@s1 }}) as [A'' [s'' [? ?]]] by mauto 2.
+    assert (exists a, {{ #| ρ[x1] |↘ ⇑! a (length Γ - x1 - 1) }}) as [? Heq] by mauto 2.
+    simplify_evals.
+
+    assert (x < length Γ) by mauto 2. 
+    assert (x1 < length Γ) by mauto 2.
+    eexists.
+    f_equal.
+Qed.
+
+#[export]
+  Hint Resolve is_typ_constr_and_typ_subtyp_var_implies_eq_var : mcpts.
 
 Theorem is_typ_constr_and_exp_eq_typ_implies_eq_typ {P} (pred_P : PredicativeSig P) : forall (Γ : ctx P) A s s',
     is_typ_constr A ->
@@ -220,10 +309,84 @@ Proof.
 Qed.
 
 #[export]
-Hint Resolve is_typ_constr_and_typ_eq_typ_implies_eq_typ : mcpts.
+  Hint Resolve is_typ_constr_and_typ_eq_typ_implies_eq_typ : mcpts.
 
 
 
+Theorem is_typ_constr_and_typ_subtyp_typ_implies_eq_typ_left {P} (pred_P : PredicativeSig P) : forall (Γ : ctx P) A s,
+    is_typ_constr A ->
+    {{ Γ ⊢ A ⊆ Sort@s }} ->
+    exists s', A = {{{ Sort@s' }}}.
+Proof.
+  intros * Histyp ?.
+  assert {{ ⟪ pred_P ⟫ Γ ⊨ A ⊆ Sort@s }} as [env_relΓ] by mauto using completeness_fundamental_typ_subtyp.
+  destruct_conjs.
+  assert (exists p p', initial_env Γ p /\ initial_env Γ p' /\ {{ Dom p ≈ p' ∈ env_relΓ }}) as [ρ [ρ' ?]] by mauto using per_ctx_then_per_env_initial_env.
+  destruct_conjs.
+  functional_initial_env_rewrite_clear.
+  (on_all_hyp: destruct_rel_by_assumption env_relΓ).
+  destruct_by_head (@rel_typ_unsorted).
+  destruct_by_head (@rel_exp).
+  invert_rel_typ_body.
+  destruct (per_subtyp_sort_inv_right pred_P H12) as [s' []].
+  inversion H5; subst.
+  
+  assert (per_typ_elem pred_P (per_sort pred_P s) d{{{ Sort@s }}} d{{{ Sort@s }}}) by (econstructor; reflexivity).
+  handle_per_typ_elem_irrel.
+  assert (is_typ_constr {{{ Sort@s }}}) as Histyp' by mauto 1.
+  dependent destruction H5.
+  - destruct Histyp; invert_rel_typ_body.
+    + eexists; reflexivity.
+    + destruct (is_typ_constr_and_var_subtyp_typ_implies_eq_var pred_P _ _ _ Histyp' H).
+      inversion H5.
+  - invert_per_sort_elem H5.
+    destruct Histyp;
+      invert_rel_typ_body.
+    + eexists; reflexivity.
+    + destruct (is_typ_constr_and_var_subtyp_typ_implies_eq_var pred_P _ _ _ Histyp' H).
+      inversion H5.
+Qed.
+
+#[export]
+  Hint Resolve is_typ_constr_and_typ_subtyp_typ_implies_eq_typ_left : mcpts.
+
+Theorem is_typ_constr_and_typ_subtyp_sort_implies_eq_typ {P} (pred_P : PredicativeSig P) : forall (Γ : ctx P) A s,
+    is_typ_constr A ->
+    {{ Γ ⊢ Sort@s ⊆ A }} ->
+    exists s', A = {{{ Sort@s' }}}.
+Proof.
+  intros * Histyp ?.
+  assert {{ ⟪ pred_P ⟫ Γ ⊨ Sort@s ⊆ A }} as [env_relΓ] by mauto using completeness_fundamental_typ_subtyp.
+  destruct_conjs.
+  assert (exists p p', initial_env Γ p /\ initial_env Γ p' /\ {{ Dom p ≈ p' ∈ env_relΓ }}) as [ρ [ρ' ?]] by mauto using per_ctx_then_per_env_initial_env.
+  destruct_conjs.
+  functional_initial_env_rewrite_clear.
+  (on_all_hyp: destruct_rel_by_assumption env_relΓ).
+  destruct_by_head (@rel_typ_unsorted).
+  destruct_by_head (@rel_exp).
+  invert_rel_typ_body.
+  destruct (per_subtyp_sort_inv_left pred_P H12) as [s' []].
+  inversion H3; subst.
+  
+  assert (per_typ_elem pred_P (per_sort pred_P s) d{{{ Sort@s }}} d{{{ Sort@s }}}) by (econstructor; reflexivity).
+  handle_per_typ_elem_irrel.
+
+  assert (is_typ_constr {{{ Sort@s }}}) as Histyp' by mauto 2.                                             
+  dependent destruction H3.
+  - destruct Histyp; invert_rel_typ_body.
+    + eexists; reflexivity.
+    + destruct (is_typ_constr_and_typ_subtyp_var_implies_eq_var pred_P _ _ _ Histyp' H).
+      inversion H5.
+  - invert_per_sort_elem H3.
+    destruct Histyp;
+      invert_rel_typ_body.
+    + eexists; reflexivity.
+    + destruct (is_typ_constr_and_typ_subtyp_var_implies_eq_var pred_P _ _ _ Histyp' H).
+      inversion H5.
+Qed.
+
+#[export]
+  Hint Resolve is_typ_constr_and_typ_subtyp_sort_implies_eq_typ : mcpts.
 
 Theorem is_typ_constr_and_exp_eq_nat_implies_eq_nat {P} (pred_P : PredicativeSig P) : forall (Γ : ctx P) A s,
     is_typ_constr A ->
@@ -283,12 +446,80 @@ Proof.
 Qed.
 
 #[export]
-Hint Resolve is_typ_constr_and_typ_eq_nat_implies_eq_nat : mcpts.
+  Hint Resolve is_typ_constr_and_typ_eq_nat_implies_eq_nat : mcpts.
+
+Theorem is_typ_constr_and_typ_subset_nat_implies_eq_nat {P} (pred_P : PredicativeSig P) : forall (Γ : ctx P) A,
+    is_typ_constr A ->
+    {{ Γ ⊢ A ⊆ ℕ }} ->
+    A = {{{ ℕ }}}.
+Proof.
+  intros * Histyp ?.
+  assert {{ ⟪ pred_P ⟫ Γ ⊨ A ⊆ ℕ }} as [env_relΓ] by mauto using completeness_fundamental_typ_subtyp.
+  destruct_conjs.
+  assert (exists p p', initial_env Γ p /\ initial_env Γ p' /\ {{ Dom p ≈ p' ∈ env_relΓ }}) as [ρ [ρ' ?]] by mauto using per_ctx_then_per_env_initial_env.
+  destruct_conjs.
+  functional_initial_env_rewrite_clear.
+  (on_all_hyp: destruct_rel_by_assumption env_relΓ).
+  destruct_by_head @rel_typ_unsorted.
+  destruct_by_head @rel_exp.
+  invert_rel_typ_body.
+
+  assert (a0 = d{{{ ℕ }}}) by (eapply per_subtyp_nat_inv_right; mauto 2).
+  subst.
+  handle_per_typ_elem_irrel.
+  
+  
+  inversion_clear H8.
+  invert_per_sort_elem H5.
+  destruct Histyp;
+    invert_rel_typ_body;
+    invert_per_sort_elems.  
+  - reflexivity.
+  - assert (is_typ_constr (@a_nat P)) as Histyp' by mauto 1.
+    destruct (is_typ_constr_and_var_subtyp_typ_implies_eq_var pred_P _ _ _ Histyp' H).
+    inversion H5.
+Qed.
+
+#[export]
+  Hint Resolve is_typ_constr_and_typ_subset_nat_implies_eq_nat : mcpts.
 
 
+Theorem is_typ_constr_and_nat_subset_typ_implies_eq_nat {P} (pred_P : PredicativeSig P) : forall (Γ : ctx P) A,
+    is_typ_constr A ->
+    {{ Γ ⊢ ℕ ⊆ A }} ->
+    A = {{{ ℕ }}}.
+Proof.
+  intros * Histyp ?.
+  assert {{ ⟪ pred_P ⟫ Γ ⊨ ℕ ⊆ A }} as [env_relΓ] by mauto using completeness_fundamental_typ_subtyp.
+  destruct_conjs.
+  assert (exists p p', initial_env Γ p /\ initial_env Γ p' /\ {{ Dom p ≈ p' ∈ env_relΓ }}) as [ρ [ρ' ?]] by mauto using per_ctx_then_per_env_initial_env.
+  destruct_conjs.
+  functional_initial_env_rewrite_clear.
+  (on_all_hyp: destruct_rel_by_assumption env_relΓ).
+  destruct_by_head @rel_typ_unsorted.
+  destruct_by_head @rel_exp.
+  invert_rel_typ_body.
 
+  assert (a = d{{{ ℕ }}}) by (eapply per_subtyp_nat_inv_left; mauto 2).
+  subst.
+  handle_per_typ_elem_irrel.
+  
+  
+  inversion_clear H8.
+  invert_per_sort_elem H3.
+  destruct Histyp;
+    invert_rel_typ_body;
+    invert_per_sort_elems.  
+  - reflexivity.
+  - assert (is_typ_constr (@a_nat P)) as Histyp' by mauto 1.
+    destruct (is_typ_constr_and_typ_subtyp_var_implies_eq_var pred_P _ _ _ Histyp' H).
+    inversion H5.
+Qed.
 
-Theorem is_typ_constr_and_exp_eq_pi_implies_eq_pi {P} (pred_P : PredicativeSig P) : forall Γ A B C s1 s2 s3 s (r : Ru P s1 s2 s3),
+#[export]
+  Hint Resolve is_typ_constr_and_nat_subset_typ_implies_eq_nat : mcpts.
+
+Theorem is_typ_constr_and_exp_eq_pi_implies_eq_pi {P} (pred_P : PredicativeSig P) : forall Γ A B C s1 s2 s3 s (r : Ru_pi P s1 s2 s3),
     is_typ_constr A ->
     {{ Γ ⊢ A ≈ Π r B C : Sort@s }} ->
     exists B' C', A = {{{ Π r B' C' }}}.
@@ -319,7 +550,7 @@ Qed.
 #[export]
 Hint Resolve is_typ_constr_and_exp_eq_pi_implies_eq_pi : mcpts.
 
-Theorem is_typ_constr_and_typ_eq_pi_implies_eq_pi {P} (pred_P : PredicativeSig P) : forall Γ A B C s1 s2 s3 (r : Ru P s1 s2 s3),
+Theorem is_typ_constr_and_typ_eq_pi_implies_eq_pi {P} (pred_P : PredicativeSig P) : forall Γ A B C s1 s2 s3 (r : Ru_pi P s1 s2 s3),
     is_typ_constr A ->
     {{ Γ ⊢ A ≈ Π r B C }} ->
     exists B' C', A = {{{ Π r B' C' }}}.
@@ -347,3 +578,64 @@ Qed.
 
 #[export]
 Hint Resolve is_typ_constr_and_typ_eq_pi_implies_eq_pi : mcpts.
+
+Theorem is_typ_constr_and_typ_subtyp_pi_implies_eq_pi {P} (pred_P : PredicativeSig P) : forall Γ A B C s1 s2 s3 (r : Ru_pi P s1 s2 s3),
+    is_typ_constr A ->
+    {{ Γ ⊢ A ⊆ Π r B C }} ->
+    exists B' C', A = {{{ Π r B' C' }}}.
+Proof.
+  intros * Histyp ?.  
+  assert {{ ⟪ pred_P ⟫ Γ ⊨ A ⊆ Π r B C }} as [env_relΓ] by mauto using completeness_fundamental_typ_subtyp.
+  destruct_conjs.
+  assert (exists p p', initial_env Γ p /\ initial_env Γ p' /\ {{ Dom p ≈ p' ∈ env_relΓ }}) as [ρ [ρ' ?]] by mauto using per_ctx_then_per_env_initial_env.
+  destruct_conjs.
+  functional_initial_env_rewrite_clear.
+  (on_all_hyp: destruct_rel_by_assumption env_relΓ).
+  destruct_by_head @rel_typ_unsorted.
+  destruct_by_head @rel_exp.
+  invert_rel_typ_body.
+
+  destruct (per_subtyp_pi_inv_right pred_P H12) as [a' [ρ' [B']]].
+  subst.
+
+  destruct Histyp;
+    invert_rel_typ_body;
+    destruct_conjs;
+    invert_per_sort_elems.  
+  - do 2 eexists. reflexivity.
+  - assert (is_typ_constr {{{ Π r B C }}}) as Histyp' by mauto 1.
+    destruct (is_typ_constr_and_var_subtyp_typ_implies_eq_var pred_P _ _ _ Histyp' H).
+    inversion H6.
+Qed.
+
+#[export]
+  Hint Resolve is_typ_constr_and_typ_subtyp_pi_implies_eq_pi : mcpts.
+
+Theorem is_typ_constr_and_pi_subtyp_typ_implies_eq_pi {P} (pred_P : PredicativeSig P) : forall Γ A B C s1 s2 s3 (r : Ru_pi P s1 s2 s3),
+    is_typ_constr A ->
+    {{ Γ ⊢ Π r B C ⊆ A }} ->
+    exists B' C', A = {{{ Π r B' C' }}}.
+Proof.
+  intros * Histyp ?.  
+  assert {{ ⟪ pred_P ⟫ Γ ⊨ Π r B C ⊆ A }} as [env_relΓ] by mauto using completeness_fundamental_typ_subtyp.
+  destruct_conjs.
+  assert (exists p p', initial_env Γ p /\ initial_env Γ p' /\ {{ Dom p ≈ p' ∈ env_relΓ }}) as [ρ [ρ' ?]] by mauto using per_ctx_then_per_env_initial_env.
+  destruct_conjs.
+  functional_initial_env_rewrite_clear.
+  (on_all_hyp: destruct_rel_by_assumption env_relΓ).
+  destruct_by_head @rel_typ_unsorted.
+  destruct_by_head @rel_exp.
+  invert_rel_typ_body.
+
+  destruct (per_subtyp_pi_inv_left pred_P H12) as [a' [ρ' [B']]].
+  subst.
+
+  destruct Histyp;
+    invert_rel_typ_body;
+    destruct_conjs;
+    invert_per_sort_elems.  
+  - do 2 eexists. reflexivity.
+  - assert (is_typ_constr {{{ Π r B C }}}) as Histyp' by mauto 1.
+    destruct (is_typ_constr_and_typ_subtyp_var_implies_eq_var pred_P _ _ _ Histyp' H).
+    inversion H6.
+Qed.
